% !TEX root = ../main.tex

% Exercises section

\section{Exercises}

\begin{enumerate}
	\item For $X: \Omega \rightarrow \mathbb{R}$ and $h: \mathbb{R} \rightarrow [a, b]$, show that $\mathbb{P}(h(X) \geq c) \geq \displaystyle\frac{b - \mathbb{E}[h(X)]}{b - c}$.
    	\newline Consider, $b - h(X) \leq (b - c) 1_{h(X) > c}$
    	\newline Taking expectation on both sides,
   	 \newline $b - \mathbb{E}[h(X)]  \leq (b - c) \mathbb{P}(h(X) \geq c)$
   	 \newline Therefore, $\mathbb{P}(h(X) \geq c) \geq \displaystyle\frac{b - \mathbb{E}[h(X)]}{b - c}$.

	\item For $X: \Omega \rightarrow \mathbb{R}$ and $h: \mathbb{R} \rightarrow [a, b]$, show that $\mathbb{P}(h(X) \geq c) \leq \displaystyle\frac{\mathbb{E}[h(X)] - a}{c - a}$.
    	\newline Consider, $h(X) - a \geq (c - a) 1_{h(X) > c}$
    	\newline Taking expectation on both sides,
   	 \newline $\mathbb{E}[h(X)] - a \geq (c - a) \mathbb{P}(h(X) \geq c)$
   	 \newline Therefore, $\mathbb{P}(h(X) \geq c) \leq \displaystyle\frac{\mathbb{E}[h(X)] - a}{c - a}$.

	
	
\end{enumerate}